

**MATHEMATICAL ANALYSIS 1**  
**HOMEWORK 11**

- (1) Using Maclaurin polynomials, determine  $\alpha \in \mathbb{R}$  so that

$$f(x) = (\arctan 2x)^2 - \alpha x \sin x$$

is infinitesimal of order 4 with respect to  $\varphi(x) = x$  as  $x \rightarrow 0$ .

- (2) Compute  $f^{(6)}(0)$  where  $f$  is the function

$$f(x) = \sinh(x^2 + 2 \sin^4 x).$$

- (3) Determine the order and the principal part as  $x \rightarrow +\infty$  with respect to  $\varphi(x) = \frac{1}{x}$  of the infinitesimal function

$$f(x) = \sqrt[3]{1 + 3x^2 + x^3} - \sqrt[5]{2 + 5x^4 + x^5}.$$

- (4) Determine the order and the principal part as  $x \rightarrow 0$  with respect to  $\varphi(x) = x$  of the infinitesimal function

$$f(x) = \sqrt[3]{1 - x^2} - \sqrt{1 - \frac{2}{3}x^2} + \sin \frac{x^4}{18}.$$

- (5) For different values of  $\alpha \in \mathbb{R}$ , as  $x \rightarrow 0$ , determine the order of the following infinitesimal function with respect to  $\varphi(x) = x$ :

$$f(x) = \ln \cos x + \ln \cosh(\alpha x).$$

- (6) Compute the following indefinite integrals using integration by parts:

(a)  $\int \cos^4 x \, dx$

(c)  $\int \ln^2 x \, dx$

(b)  $\int \ln(\sqrt[3]{1 + x^2}) \, dx$

(d)  $\int x \arctan x \, dx$

- (7) Compute  $\int \frac{1}{(1+x^2)^2} \, dx$ . [Hint: compute  $\int \frac{1}{1+x^2} \, dx$  using integration by parts with  $f(x) = \frac{1}{1+x^2}$  and  $g'(x) = 1$ .]

- (8) Compute the following indefinite integrals using substitution:

(a)  $\int \frac{e^{2x}}{e^x + 1} \, dx$

(c)  $\int \frac{1}{\sinh x} \, dx$

(b)  $\int \frac{1 + \cos x}{1 - \cos x} \, dx$

(d)  $\int \frac{1}{e^{4x} + 1} \, dx$

- (9) (a) Recall what the *derivatives* of  $\arctan x$  and of  $\arctan \frac{1}{x}$  are.  
(b) Use the previous part to prove that

$$\arctan \frac{1}{x} = \frac{\pi}{2} - \arctan x, \quad \forall x > 0.$$

# HOMEWORK 11 SOLUTIONS

## (1) Determine $\alpha$ so that $f(x)$ is infinitesimal of order 4

We want  $f(x) = (\arctan 2x)^2 - \alpha x \sin x = O(x^4)$  as  $x \rightarrow 0$ , but with the coefficients of  $x$ ,  $x^2$ ,  $x^3$  all zero. Compute Maclaurin expansions up to order 4.

First,  $\arctan u = u - \frac{u^3}{3} + o(u^3)$ . With  $u = 2x$ :

$$\arctan 2x = 2x - \frac{(2x)^3}{3} + o(x^3) = 2x - \frac{8x^3}{3} + o(x^3).$$

Square this:

$$\begin{aligned} (\arctan 2x)^2 &= \left(2x - \frac{8}{3}x^3 + o(x^3)\right)^2 \\ &= (2x)^2 + 2(2x)\left(-\frac{8}{3}x^3\right) + o(x^4) \\ &= 4x^2 - \frac{32}{3}x^4 + o(x^4). \end{aligned}$$

Note: the cross term gives  $x^4$ , and there is no  $x^3$  term because the expansion of  $\arctan 2x$  has no  $x^2$  term.

$$\text{Next, } x \sin x = x \left(x - \frac{x^3}{6} + o(x^3)\right) = x^2 - \frac{x^4}{6} + o(x^4).$$

Thus

$$f(x) = \left(4x^2 - \frac{32}{3}x^4 + o(x^4)\right) - \alpha \left(x^2 - \frac{x^4}{6} + o(x^4)\right) = (4 - \alpha)x^2 + \left(-\frac{32}{3} + \frac{\alpha}{6}\right)x^4 + o(x^4).$$

For  $f(x)$  to be infinitesimal of order 4, the coefficients of  $x^2$  and  $x^3$  (if any) must vanish. There is no  $x^3$  term. So we require:

$$4 - \alpha = 0 \quad \Rightarrow \quad \alpha = 4.$$

With  $\alpha = 4$ , the  $x^4$  coefficient becomes:

$$-\frac{32}{3} + \frac{4}{6} = -\frac{32}{3} + \frac{2}{3} = -\frac{30}{3} = -10 \neq 0.$$

Thus  $f(x) = -10x^4 + o(x^4)$ , which is indeed infinitesimal of order 4.

**Answer:**  $\alpha = 4$ .

## (2) Compute $f^{(6)}(0)$ for $f(x) = \sinh(x^2 + 2 \sin^4 x)$

Recall that for an analytic function, the coefficient of  $x^6$  in its Maclaurin expansion is  $\frac{f^{(6)}(0)}{6!}$ . So we need the expansion of  $f(x)$  up to  $x^6$ .

First, expand  $\sin^4 x$ . We know  $\sin x = x - \frac{x^3}{6} + \frac{x^5}{120} + o(x^5)$ . Compute  $\sin^4 x = (\sin x)^4$  up to  $x^6$ . It's easier to compute step by step:

$$\begin{aligned} \sin x &= x - \frac{x^3}{6} + \frac{x^5}{120} + o(x^5). \\ \sin^2 x &= \left(x - \frac{x^3}{6} + \frac{x^5}{120} + o(x^5)\right)^2 \\ &= x^2 - 2x \cdot \frac{x^3}{6} + \left(\frac{x^6}{36} + 2x \cdot \frac{x^5}{120}\right) + \dots \quad (\text{keeping up to } x^6) \\ &= x^2 - \frac{1}{3}x^4 + \left(\frac{1}{36} + \frac{1}{60}\right)x^6 + o(x^6) \\ &= x^2 - \frac{1}{3}x^4 + \left(\frac{5}{180} + \frac{3}{180}\right)x^6 + o(x^6) \\ &= x^2 - \frac{1}{3}x^4 + \frac{8}{180}x^6 + o(x^6) \\ &= x^2 - \frac{1}{3}x^4 + \frac{2}{45}x^6 + o(x^6). \end{aligned}$$

Then

$$\begin{aligned}\sin^4 x &= (\sin^2 x)^2 = \left(x^2 - \frac{1}{3}x^4 + \frac{2}{45}x^6 + o(x^6)\right)^2 \\ &= (x^2)^2 + 2x^2 \left(-\frac{1}{3}x^4\right) + \left(2x^2 \cdot \frac{2}{45}x^6 + \left(-\frac{1}{3}x^4\right)^2\right) + o(x^6) \\ &= x^4 - \frac{2}{3}x^6 + \left(\frac{4}{45}x^8 + \frac{1}{9}x^8\right) + o(x^6).\end{aligned}$$

Terms with  $x^8$  are  $o(x^6)$ , so we only keep up to  $x^6$ :

$$\sin^4 x = x^4 - \frac{2}{3}x^6 + o(x^6).$$

Now compute  $u(x) = x^2 + 2\sin^4 x$ :

$$u(x) = x^2 + 2\left(x^4 - \frac{2}{3}x^6 + o(x^6)\right) = x^2 + 2x^4 - \frac{4}{3}x^6 + o(x^6).$$

Next, expand  $\sinh u = u + \frac{u^3}{6} + \frac{u^5}{120} + o(u^5)$ . We need up to  $u^6$  in  $x$ . Since  $u = O(x^2)$ , terms up to  $x^6$  come from  $u$ ,  $\frac{u^3}{6}$  (since  $u^3 = O(x^6)$ ), and possibly  $\frac{u^5}{120}$  which is  $O(x^{10})$ , negligible.

So:

$$f(x) = u + \frac{u^3}{6} + o(x^6).$$

Compute  $u^3$  up to  $x^6$ :

$$\begin{aligned}u &= x^2 + 2x^4 - \frac{4}{3}x^6 + o(x^6), \\ u^3 &= (x^2)^3 + 3(x^2)^2(2x^4) + o(x^6) \quad (\text{other terms are } O(x^8) \text{ or higher}) \\ &= x^6 + 6x^8 + o(x^6) = x^6 + o(x^6).\end{aligned}$$

Thus  $\frac{u^3}{6} = \frac{x^6}{6} + o(x^6)$ .

Therefore:

$$f(x) = \left(x^2 + 2x^4 - \frac{4}{3}x^6\right) + \frac{1}{6}x^6 + o(x^6) = x^2 + 2x^4 + \left(-\frac{4}{3} + \frac{1}{6}\right)x^6 + o(x^6).$$

Compute  $-\frac{4}{3} + \frac{1}{6} = -\frac{8}{6} + \frac{1}{6} = -\frac{7}{6}$ .

Hence

$$f(x) = x^2 + 2x^4 - \frac{7}{6}x^6 + o(x^6).$$

The coefficient of  $x^6$  is  $-\frac{7}{6}$ . But the Maclaurin coefficient is  $\frac{f^{(6)}(0)}{6!}$ , so:

$$\frac{f^{(6)}(0)}{6!} = -\frac{7}{6} \Rightarrow f^{(6)}(0) = -\frac{7}{6} \cdot 720 = -840.$$

**Answer:**  $f^{(6)}(0) = -840$ .

(3) **Order and principal part as  $x \rightarrow +\infty$  with respect to  $\varphi(x) = 1/x$**

We consider  $f(x)$  as  $x \rightarrow +\infty$ . We substitute  $t = 1/x$ , so  $t \rightarrow 0^+$ .

$$\begin{aligned}\sqrt[3]{1 + 3x^2 + x^3} &= x\sqrt[3]{\frac{1}{x^3} + \frac{3}{x} + 1} = x\sqrt[3]{1 + 3t + t^3}, \\ \sqrt[5]{2 + 5x^4 + x^5} &= x\sqrt[5]{\frac{2}{x^5} + \frac{5}{x} + 1} = x\sqrt[5]{1 + 5t + 2t^5}.\end{aligned}$$

Thus

$$f(x) = x \left( \sqrt[3]{1 + 3t + t^3} - \sqrt[5]{1 + 5t + 2t^5} \right), \quad t = 1/x.$$

We use the binomial expansion  $(1 + u)^a = 1 + au + \frac{a(a-1)}{2}u^2 + o(u^2)$ . We must expand up to the  $t^2$  term since the  $t$  terms are expected to cancel.

**First Term Expansion (up to  $o(t^2)$ ).** For  $\sqrt[3]{1+3t+t^3}$ , let  $u = 3t + t^3$  and  $a = 1/3$ . The  $t^2$  coefficient is governed by the  $u^2$  term,  $u^2 = (3t)^2 + O(t^4) = 9t^2 + O(t^4)$ .

$$\begin{aligned}(1+u)^{1/3} &= 1 + \frac{1}{3}u + \frac{\frac{1}{3}(-\frac{2}{3})}{2}u^2 + o(u^2) \\ &= 1 + \frac{1}{3}(3t + t^3) - \frac{1}{9}(9t^2) + o(t^2) \\ &= 1 + t - t^2 + o(t^2).\end{aligned}$$

**Second Term Expansion (up to  $o(t^2)$ ).** For  $\sqrt[5]{1+5t+2t^5}$ , let  $v = 5t + 2t^5$  and  $a = 1/5$ . The  $t^2$  coefficient is governed by the  $v^2$  term,  $v^2 = (5t)^2 + O(t^6) = 25t^2 + O(t^6)$ .

$$\begin{aligned}(1+v)^{1/5} &= 1 + \frac{1}{5}v + \frac{\frac{1}{5}(-\frac{4}{5})}{2}v^2 + o(v^2) \\ &= 1 + \frac{1}{5}(5t + 2t^5) - \frac{2}{25}(25t^2) + o(t^2) \\ &= 1 + t - 2t^2 + o(t^2).\end{aligned}$$

**Calculating the Difference.**

$$\begin{aligned}\sqrt[3]{1+3t+t^3} - \sqrt[5]{1+5t+2t^5} &= (1+t-t^2+o(t^2)) - (1+t-2t^2+o(t^2)) \\ &= (1-1) + (t-t) + (-t^2 - (-2t^2)) + o(t^2) \\ &= 0 + 0 + (-t^2 + 2t^2) + o(t^2) \\ &= t^2 + o(t^2).\end{aligned}$$

Therefore,

$$f(x) = x \cdot (t^2 + o(t^2)) = x \cdot \left(\frac{1}{x}\right)^2 + o\left(x \cdot \frac{1}{x^2}\right) = \frac{1}{x} + o\left(\frac{1}{x}\right).$$

Hence, as  $x \rightarrow +\infty$ ,  $f(x) \sim \frac{1}{x}$ .

**Order:** 1 (since  $f(x) = O(1/x)$ ).

**Principal part:**  $\frac{1}{x}$ .

(4) **Order and principal part as  $x \rightarrow 0$  with respect to  $\varphi(x) = x$**

We expand each term up to sufficient order.

$$\text{First, } \sqrt[3]{1-x^2} = (1-x^2)^{1/3} = 1 - \frac{1}{3}x^2 + \frac{\frac{1}{3}(-\frac{2}{3})}{2}x^4 + o(x^4) = 1 - \frac{1}{3}x^2 - \frac{1}{9}x^4 + o(x^4).$$

$$\text{Second, } \sqrt{1-\frac{2}{3}x^2} = (1-\frac{2}{3}x^2)^{1/2} = 1 - \frac{1}{2} \cdot \frac{2}{3}x^2 + \frac{\frac{1}{2}(-\frac{1}{2})}{2} \left(\frac{2}{3}x^2\right)^2 + o(x^4) = 1 - \frac{1}{3}x^2 - \frac{1}{18}x^4 + o(x^4).$$

$$\text{Third, } \sin \frac{x^4}{18} = \frac{x^4}{18} + o(x^4).$$

Now compute:

$$\begin{aligned}\sqrt[3]{1-x^2} - \sqrt{1-\frac{2}{3}x^2} &= \left(1 - \frac{1}{3}x^2 - \frac{1}{9}x^4\right) - \left(1 - \frac{1}{3}x^2 - \frac{1}{18}x^4\right) + o(x^4) \\ &= \left(-\frac{1}{9} + \frac{1}{18}\right)x^4 + o(x^4) = -\frac{1}{18}x^4 + o(x^4).\end{aligned}$$

Then add  $\sin \frac{x^4}{18}$ :

$$f(x) = -\frac{1}{18}x^4 + \frac{1}{18}x^4 + o(x^4) = o(x^4).$$

So the  $x^4$  terms cancel. We need to go to higher order to find the leading term.

Compute expansions to  $x^6$ :

$$\begin{aligned}\sqrt[3]{1-x^2} &= 1 - \frac{1}{3}x^2 - \frac{1}{9}x^4 + \frac{\frac{1}{3}(-\frac{2}{3})(-\frac{5}{3})}{6}x^6 + o(x^6). \text{ Compute the } x^6 \text{ coefficient: } \frac{(1/3)(-2/3)(-5/3)}{6} = \\ \frac{(10/27)}{6} &= \frac{10}{162} = \frac{5}{81}. \text{ Thus } \sqrt[3]{1-x^2} = 1 - \frac{1}{3}x^2 - \frac{1}{9}x^4 + \frac{5}{81}x^6 + o(x^6).\end{aligned}$$

$\sqrt{1 - \frac{2}{3}x^2} = 1 - \frac{1}{3}x^2 - \frac{1}{18}x^4 + \frac{\frac{1}{2}(-\frac{1}{2})(-\frac{3}{2})}{6} \left(\frac{2}{3}x^2\right)^3 + o(x^6)$ . Compute the  $x^6$  coefficient:  $\frac{(1/2)(-1/2)(-3/2)}{6}$ .  
 $\left(\frac{2}{3}\right)^3 = \frac{(3/8)}{6} \cdot \frac{8}{27} = \frac{1}{16} \cdot \frac{8}{27} = \frac{1}{54}$ . Thus  $\sqrt{1 - \frac{2}{3}x^2} = 1 - \frac{1}{3}x^2 - \frac{1}{18}x^4 - \frac{1}{54}x^6 + o(x^6)$ .

$$\sin \frac{x^4}{18} = \frac{x^4}{18} - \frac{1}{6} \left(\frac{x^4}{18}\right)^3 + \cdots = \frac{x^4}{18} + o(x^6).$$

Now combine:

$$\begin{aligned} \sqrt[3]{1-x^2} - \sqrt{1 - \frac{2}{3}x^2} &= \left(1 - \frac{1}{3}x^2 - \frac{1}{9}x^4 + \frac{5}{81}x^6\right) - \left(1 - \frac{1}{3}x^2 - \frac{1}{18}x^4 - \frac{1}{54}x^6\right) + o(x^6) \\ &= \left(-\frac{1}{9} + \frac{1}{18}\right)x^4 + \left(\frac{5}{81} + \frac{1}{54}\right)x^6 + o(x^6) \\ &= -\frac{1}{18}x^4 + \left(\frac{10}{162} + \frac{3}{162}\right)x^6 + o(x^6) \\ &= -\frac{1}{18}x^4 + \frac{13}{162}x^6 + o(x^6). \end{aligned}$$

Add  $\sin \frac{x^4}{18}$ :

$$f(x) = \left(-\frac{1}{18}x^4 + \frac{13}{162}x^6\right) + \frac{1}{18}x^4 + o(x^6) = \frac{13}{162}x^6 + o(x^6).$$

Thus  $f(x) \sim \frac{13}{162}x^6$  as  $x \rightarrow 0$ .

**Order:** 6.

**Principal part:**  $\frac{13}{162}x^6$ .

- (5) **Determine the order of the infinitesimal function**  $f(x) = \ln \cos x + \ln \cosh(\alpha x)$  **with respect to**  $\varphi(x) = x$  **as**  $x \rightarrow 0$ , **for different values of**  $\alpha \in \mathbb{R}$ .

1. *Maclaurin Expansions of Individual Components.* We use the known Maclaurin expansions for  $\cos x$  and  $\cosh u$  with Peano's remainder up to order 4:

$$\begin{aligned} \cos x &= 1 - \frac{x^2}{2} + \frac{x^4}{24} + o(x^5) \\ \cosh u &= 1 + \frac{u^2}{2} + \frac{u^4}{24} + o(u^5) \end{aligned}$$

Substitute  $u = \alpha x$  into the cosh expansion:

$$\cosh(\alpha x) = 1 + \frac{\alpha^2 x^2}{2} + \frac{\alpha^4 x^4}{24} + o(x^5).$$

Now we use the expansion  $\ln(1+u) = u - \frac{u^2}{2} + o(u^2)$ .

2. *Expansion of  $\ln(\cos x)$ .* Let  $u_1 = \cos x - 1 = -\frac{x^2}{2} + \frac{x^4}{24} + o(x^5)$ . Since  $u_1$  starts with  $x^2$ , we need the expansion up to  $u_1^2$  to get terms up to  $x^4$ .

$$\begin{aligned} \ln(\cos x) &= \ln(1+u_1) = u_1 - \frac{1}{2}u_1^2 + o(u_1^2) \\ &= \left(-\frac{x^2}{2} + \frac{x^4}{24}\right) - \frac{1}{2}\left(-\frac{x^2}{2} + \frac{x^4}{24}\right)^2 + o(x^4) \\ &= -\frac{x^2}{2} + \frac{x^4}{24} - \frac{1}{2}\left(\frac{x^4}{4} + o(x^6)\right) + o(x^4) \\ &= -\frac{x^2}{2} + \frac{x^4}{24} - \frac{x^4}{8} + o(x^4) \\ &= -\frac{x^2}{2} + \left(\frac{1}{24} - \frac{3}{24}\right)x^4 + o(x^4) \\ &= -\frac{x^2}{2} - \frac{1}{12}x^4 + o(x^4). \end{aligned}$$

3. *Expansion of  $\ln(\cosh(\alpha x))$ .* Let  $u_2 = \cosh(\alpha x) - 1 = \frac{\alpha^2 x^2}{2} + \frac{\alpha^4 x^4}{24} + o(x^5)$ . Again, we expand up to  $u_2^2$  to get terms up to  $x^4$ .

$$\begin{aligned}\ln(\cosh(\alpha x)) &= \ln(1 + u_2) = u_2 - \frac{1}{2}u_2^2 + o(u_2^2) \\ &= \left(\frac{\alpha^2 x^2}{2} + \frac{\alpha^4 x^4}{24}\right) - \frac{1}{2}\left(\frac{\alpha^2 x^2}{2} + \frac{\alpha^4 x^4}{24}\right)^2 + o(x^4) \\ &= \frac{\alpha^2 x^2}{2} + \frac{\alpha^4 x^4}{24} - \frac{1}{2}\left(\frac{\alpha^4 x^4}{4} + o(x^6)\right) + o(x^4) \\ &= \frac{\alpha^2 x^2}{2} + \frac{\alpha^4 x^4}{24} - \frac{\alpha^4 x^4}{8} + o(x^4) \\ &= \frac{\alpha^2 x^2}{2} + \left(\frac{1}{24} - \frac{3}{24}\right)\alpha^4 x^4 + o(x^4) \\ &= \frac{\alpha^2 x^2}{2} - \frac{\alpha^4}{12}x^4 + o(x^4).\end{aligned}$$

4. *Combining Terms and Determining Order.* We add the two expansions:

$$\begin{aligned}f(x) &= \ln \cos x + \ln \cosh(\alpha x) \\ &= \left(-\frac{x^2}{2} + \left(\frac{1}{24} - \frac{1}{8}\right)x^4\right) + \left(\frac{\alpha^2 x^2}{2} + \left(\frac{1}{24} - \frac{1}{8}\right)\alpha^4 x^4\right) + o(x^4) \\ &= \left(\frac{\alpha^2}{2} - \frac{1}{2}\right)x^2 + \left[\left(\frac{1}{24} - \frac{1}{8}\right)x^4 + \left(\frac{1}{24} - \frac{1}{8}\right)\alpha^4 x^4\right] + o(x^4) \\ &= \frac{1}{2}(\alpha^2 - 1)x^2 + \left(\frac{1}{4!} - \frac{1}{8}\right)(1 + \alpha^4)x^4 + o(x^4).\end{aligned}$$

We analyze the coefficient of the leading term,  $\frac{1}{2}(\alpha^2 - 1)$ .

- **Case 1:**  $\alpha^2 - 1 \neq 0$  (i.e.,  $\alpha \neq 1$  and  $\alpha \neq -1$ ) The leading term is  $\frac{1}{2}(\alpha^2 - 1)x^2$ .

$$f(x) \sim \frac{1}{2}(\alpha^2 - 1)x^2 \quad \text{as } x \rightarrow 0.$$

The order of  $f(x)$  with respect to  $\varphi(x) = x$  is **2**.

- **Case 2:**  $\alpha = 1$  or  $\alpha = -1$  If  $\alpha^2 = 1$ , the  $x^2$  term cancels. We use the fact that  $\left(\frac{1}{4!} - \frac{1}{8}\right) = -\frac{1}{12}$ .

$$f(x) = 0 \cdot x^2 + \left(-\frac{1}{12}\right)(1 + 1^4)x^4 + o(x^4) = -\frac{2}{12}x^4 + o(x^4) = -\frac{1}{6}x^4 + o(x^4).$$

$$f(x) \sim -\frac{1}{6}x^4 \quad \text{as } x \rightarrow 0.$$

The order of  $f(x)$  with respect to  $\varphi(x) = x$  is **4**.

#### (6) Indefinite integrals by parts

(a)  $\int \cos^4 x \, dx$ .

Using integration by parts: let  $f(x) = \cos^3 x$  and  $g'(x) = \cos x$ . Then  $f'(x) = -3\cos^2 x \sin x$  and  $g(x) = \sin x$ . Thus:

$$\int \cos^4 x \, dx = \cos^3 x \sin x + 3 \int \cos^2 x \sin^2 x \, dx.$$

Now,  $\sin^2 x = 1 - \cos^2 x$ , so  $\cos^2 x \sin^2 x = \cos^2 x - \cos^4 x$ . Hence:

$$\int \cos^4 x \, dx = \cos^3 x \sin x + 3 \int (\cos^2 x - \cos^4 x) \, dx.$$

Let  $I = \int \cos^4 x \, dx$ . Then:

$$I = \cos^3 x \sin x + 3 \int \cos^2 x \, dx - 3I \quad \Rightarrow \quad 4I = \cos^3 x \sin x + 3 \int \cos^2 x \, dx.$$

We compute  $\int \cos^2 x \, dx = \int \frac{1+\cos 2x}{2} \, dx = \frac{x}{2} + \frac{\sin 2x}{4} + C$ . Therefore:

$$4I = \cos^3 x \sin x + 3 \left( \frac{x}{2} + \frac{\sin 2x}{4} \right) + C.$$

Thus:

$$I = \frac{1}{4} \cos^3 x \sin x + \frac{3x}{8} + \frac{3 \sin 2x}{16} + C.$$

This is the result using integration by parts. (One may also express it as  $\frac{3x}{8} + \frac{1}{4} \sin 2x + \frac{1}{32} \sin 4x + C$  using trigonometric identities.)

(b)  $\int \ln(\sqrt[3]{1+x^2}) \, dx = \frac{1}{3} \int \ln(1+x^2) \, dx.$

Integrate by parts: let  $f(x) = \ln(1+x^2)$  and  $g'(x) = 1$ , so  $f'(x) = \frac{2x}{1+x^2}$  and  $g(x) = x$ . Then

$$\int \ln(1+x^2) \, dx = x \ln(1+x^2) - \int \frac{2x^2}{1+x^2} \, dx.$$

Now  $\frac{2x^2}{1+x^2} = 2 - \frac{2}{1+x^2}$ . Thus

$$\int \frac{2x^2}{1+x^2} \, dx = \int 2 \, dx - 2 \int \frac{1}{1+x^2} \, dx = 2x - 2 \arctan x.$$

Hence

$$\int \ln(1+x^2) \, dx = x \ln(1+x^2) - 2x + 2 \arctan x + C.$$

Therefore,

$$\int \ln(\sqrt[3]{1+x^2}) \, dx = \frac{1}{3} (x \ln(1+x^2) - 2x + 2 \arctan x) + C.$$

(c)  $\int \ln^2 x \, dx.$

Integrate by parts: let  $f(x) = \ln^2 x$  and  $g'(x) = 1$ , so  $f'(x) = 2 \ln x \cdot \frac{1}{x}$  and  $g(x) = x$ . Then

$$\int \ln^2 x \, dx = x \ln^2 x - \int 2 \ln x \, dx.$$

Now  $\int \ln x \, dx = x \ln x - x + C$ . So

$$\int \ln^2 x \, dx = x \ln^2 x - 2(x \ln x - x) + C = x \ln^2 x - 2x \ln x + 2x + C.$$

(d)  $\int x \arctan x \, dx.$

Integrate by parts: let  $f(x) = \arctan x$  and  $g'(x) = x$ , so  $f'(x) = \frac{1}{1+x^2}$  and  $g(x) = \frac{x^2}{2}$ . Then

$$\int x \arctan x \, dx = \frac{x^2}{2} \arctan x - \int \frac{x^2}{2(1+x^2)} \, dx.$$

Now  $\frac{x^2}{1+x^2} = 1 - \frac{1}{1+x^2}$ . Thus

$$\int \frac{x^2}{1+x^2} \, dx = \int 1 \, dx - \int \frac{1}{1+x^2} \, dx = x - \arctan x.$$

Hence

$$\int x \arctan x \, dx = \frac{x^2}{2} \arctan x - \frac{1}{2} (x - \arctan x) + C = \frac{1}{2} (x^2 + 1) \arctan x - \frac{x}{2} + C.$$

(7)  $\int \frac{1}{(1+x^2)^2} \, dx.$

Following the hint, first compute  $\int \frac{1}{1+x^2} \, dx$  by parts with  $f(x) = \frac{1}{1+x^2}$ ,  $g'(x) = 1$ . Then  $f'(x) = -\frac{2x}{(1+x^2)^2}$ ,  $g(x) = x$ . So

$$\int \frac{1}{1+x^2} \, dx = \frac{x}{1+x^2} + \int \frac{2x^2}{(1+x^2)^2} \, dx.$$

But note  $\frac{2x^2}{(1+x^2)^2} = \frac{2(1+x^2)-2}{(1+x^2)^2} = \frac{2}{1+x^2} - \frac{2}{(1+x^2)^2}$ . Thus

$$\int \frac{1}{1+x^2} dx = \frac{x}{1+x^2} + 2 \int \frac{1}{1+x^2} dx - 2 \int \frac{1}{(1+x^2)^2} dx.$$

Rearranging:

$$\int \frac{1}{1+x^2} dx - 2 \int \frac{1}{1+x^2} dx = \frac{x}{1+x^2} - 2 \int \frac{1}{(1+x^2)^2} dx,$$

so

$$- \int \frac{1}{1+x^2} dx = \frac{x}{1+x^2} - 2 \int \frac{1}{(1+x^2)^2} dx.$$

Thus

$$2 \int \frac{1}{(1+x^2)^2} dx = \frac{x}{1+x^2} + \int \frac{1}{1+x^2} dx = \frac{x}{1+x^2} + \arctan x + C.$$

Therefore,

$$\int \frac{1}{(1+x^2)^2} dx = \frac{1}{2} \left( \frac{x}{1+x^2} + \arctan x \right) + C.$$

### (8) Indefinite integrals by substitution

(a)  $\int \frac{e^{2x}}{e^x+1} dx$ .

Let  $y = e^x$ , so  $dy = e^x dx$ , and  $e^{2x} = y^2$ . Then

$$\int \frac{e^{2x}}{e^x+1} dx = \int \frac{y^2}{y+1} \cdot \frac{dy}{y} = \int \frac{y}{y+1} dy = \int \left( 1 - \frac{1}{y+1} \right) dy = y - \ln|y+1| + C = e^x - \ln(e^x+1) + C.$$

(b)  $\int \frac{1+\cos x}{1-\cos x} dx$ .

Let  $t = \tan(x/2)$ , then  $\cos x = \frac{1-t^2}{1+t^2}$ ,  $dx = \frac{2}{1+t^2} dt$ . Then

$$\frac{1+\cos x}{1-\cos x} = \frac{1+\frac{1-t^2}{1+t^2}}{1-\frac{1-t^2}{1+t^2}} = \frac{\frac{2}{1+t^2}}{\frac{2t^2}{1+t^2}} = \frac{1}{t^2}.$$

Thus

$$\int \frac{1+\cos x}{1-\cos x} dx = \int \frac{1}{t^2} \cdot \frac{2}{1+t^2} dt = 2 \int \frac{1}{t^2(1+t^2)} dt = 2 \int \left( \frac{1}{t^2} - \frac{1}{1+t^2} \right) dt = 2 \left( -\frac{1}{t} - \arctan t \right) + C.$$

Substitute back  $t = \tan(x/2)$ :

$$= -2 \cot(x/2) - 2 \arctan(\tan(x/2)) + C = -2 \cot(x/2) - x + C.$$

(c)  $\int \frac{1}{\sinh x} dx$ .

Recall  $\sinh x = \frac{e^x - e^{-x}}{2}$ . Multiply numerator and denominator by  $e^x$ :

$$\int \frac{1}{\sinh x} dx = \int \frac{2}{e^x - e^{-x}} dx = \int \frac{2e^x}{e^{2x} - 1} dx.$$

Let  $y = e^x$ , so  $dy = e^x dx$ . Then

$$\int \frac{2e^x}{e^{2x} - 1} dx = \int \frac{2}{y^2 - 1} dy = \int \left( \frac{1}{y-1} - \frac{1}{y+1} \right) dy = \ln|y-1| - \ln|y+1| + C = \ln \left| \frac{e^x - 1}{e^x + 1} \right| + C.$$

(d)  $\int \frac{1}{e^{4x}+1} dx$ .

Let  $y = e^{4x}$ , then  $dy = 4e^{4x} dx = 4y dx$ , so  $dx = \frac{dy}{4y}$ . Then

$$\int \frac{1}{e^{4x}+1} dx = \int \frac{1}{y+1} \cdot \frac{dy}{4y} = \frac{1}{4} \int \frac{1}{y(y+1)} dy.$$

Using partial fractions:  $\frac{1}{y(y+1)} = \frac{1}{y} - \frac{1}{y+1}$ . Thus

$$\frac{1}{4} \int \left( \frac{1}{y} - \frac{1}{y+1} \right) dy = \frac{1}{4} (\ln|y| - \ln|y+1|) + C = \frac{1}{4} \ln \left| \frac{y}{y+1} \right| + C.$$



Substitute back  $y = e^{4x}$ :

$$= \frac{1}{4} \ln \left( \frac{e^{4x}}{e^{4x} + 1} \right) + C = \frac{1}{4} \ln \left( 1 - \frac{1}{e^{4x} + 1} \right) + C = x - \frac{1}{4} \ln(e^{4x} + 1) + C.$$

(9) (a) Derivatives:

$$\frac{d}{dx} \arctan x = \frac{1}{1+x^2}, \quad \frac{d}{dx} \arctan \frac{1}{x} = \frac{1}{1+(1/x)^2} \cdot \left( -\frac{1}{x^2} \right) = -\frac{1}{x^2+1}.$$

(b) Proof of identity.

Let  $h(x) = \arctan \frac{1}{x} + \arctan x$  for  $x > 0$ . Then

$$h'(x) = -\frac{1}{1+x^2} + \frac{1}{1+x^2} = 0.$$

Thus  $h(x)$  is constant on  $(0, \infty)$ . To find the constant, evaluate at  $x = 1$ :

$$h(1) = \arctan 1 + \arctan 1 = \frac{\pi}{4} + \frac{\pi}{4} = \frac{\pi}{2}.$$

Hence for all  $x > 0$ ,

$$\arctan \frac{1}{x} + \arctan x = \frac{\pi}{2} \quad \Rightarrow \quad \arctan \frac{1}{x} = \frac{\pi}{2} - \arctan x.$$